Add record update rule

rocq-osiris/theories/program_logic/rules/record_rules.v
@@ -7,9 +7,7 @@ From osiris.logic Require Import list_z big_opLZ.
 
 (** This file defines record resource predicates and [imp] rules for record expressions. *)
 
-Section record_resources.
-
-  Context `{!osirisGS Σ}.
+Section types_helpers.
 
   Fixpoint to_vals {τ : types} : τ-#> list val :=
     match τ with
@@ -17,6 +15,9 @@ Section record_resources.
     | @type_nel.Tcons X H b =>
       λ (x : X), @tbind _ b (λ tt, #x :: (to_vals tt))
     end.
+
+  Global Instance observe_types (τ : types) : Observe τ (list val) :=
+    { observe τ := to_vals τ }.
 
   Fixpoint length (τ : types) : Z :=
     match τ with
@@ -31,61 +32,6 @@ Section record_resources.
     - intros x. simpl. unfold tapp. by rewrite length_singleton.
     - intros (x & xs). simpl. rewrite tapp_bind. length.
       rewrite IHτ. lia.
-  Qed.
-
-  Definition ownRecord {τ : types} (r : record) dq (t : mut_tag) (xs : τ) : iProp Σ :=
-    ∃ ls, isBlockLocs r ls ∗ r ⤇{dq} t ∗
-      [∗ listZ] l;v ∈ ls; (to_vals xs), l ↦{dq} v.
-
-End record_resources.
-
-Section records_reasoning.
-
-  Context `{!osirisGS Σ}.
-
-  Context {η : env} {E : coPset} {Ψ : iEff Σ}.
-
-  Lemma imp_as_record {ζ} {Φ : record → iProp Σ} (m : microvx) :
-    imp m @ E <|Ψ|> ⟨⟨ ζ ⟩⟩ {{ Φ }} -∗
-    impure E (as_record m) Ψ ζ Φ.
-  Proof.
-    iIntros "Hm".
-    iApply (imp_bind with "Hm").
-    iIntros (r) "HΦ".
-    iApply (imp_ret with "HΦ"). encode.
-  Qed.
-
-  Global Instance observe_types (τ : types) : Observe τ (list val) :=
-    { observe τ := to_vals τ }.
-
-  Global Instance notval_listloc : NotVal (list loc) := {}.
-  Local Instance notval_listval : NotVal (list val) := {}.
-
-  Lemma imp_ERecord {τ : types} {ζ} (Φs : τ -#> iProp Σ) t es :
-    ⌜length τ ≤ max_array_length⌝ -∗
-    impure E (evals η es) Ψ ζ Φs -∗
-    impure E (eval η (ERecord t es)) Ψ ζ
-      (λ r, ∃ (xs : τ), ownRecord r (DfracOwn 1) t xs ∗ Φs xs).
-  Proof.
-    iIntros "%Hlength Hes". simpl_eval.
-    iApply (imp_bind with "Hes").
-    iIntros (xs) "HΦs".
-    iApply imp_bind.
-    { simpl.
-      replace (to_vals xs) with
-      (@observe (list val) (list val) (@observe_list val Encode_val) (to_vals xs)).
-      iApply (@imp_allocn _ _ _ _ _ val Encode_val (λ ls, [∗ listZ] l;v ∈ ls; (to_vals xs), l ↦ v)%I (to_vals xs)).
-      iIntros "!>" (ls) "$".
-      simpl. rewrite map_id. reflexivity. }
-    iIntros (ls) "Hls".
-    iPoseProof (big_sepLZ2_length with "Hls") as "%Hlength_ls".
-    iApply imp_bind.
-    { iApply imp_alloc_block.
-      iPureIntro. simpl.
-      rewrite Hlength_ls. rewrite to_vals_length. assumption. }
-    iIntros (r) "(Hmut & Hblocks)".
-    iApply imp_ret. encode.
-    iFrame.
   Qed.
 
   Instance types_lookup : Lookup Z Type types :=
@@ -137,8 +83,6 @@ Section records_reasoning.
     - exact (tau_lookup_go τ (Z.to_nat f) xs).
   Defined.
 
-  Notation "xs !!τ f" := (τ_lookup_total f xs) (at level 20).
-
   Global Instance encode_types_lookup {τ : types} {f : Z} : Encode (τ !!! f).
   Proof.
     unfold lookup_total, types_lookup_total.
@@ -180,12 +124,118 @@ Section records_reasoning.
   Qed.
 
   Lemma lookup_total_to_vals {τ : types} (xs : τ) (f : Z) :
-    (to_vals xs) !!! f = #(xs !!τ f).
+    (to_vals xs) !!! f = #(τ_lookup_total f xs).
   Proof.
-    unfold "!!τ", τ_lookup_total, encode_types_lookup, lookup_total, types_lookup_total, listz_lookup_total.
+    unfold τ_lookup_total, encode_types_lookup, lookup_total, types_lookup_total, listz_lookup_total.
     case_decide as Hlt. { reflexivity. }
     generalize (Z.to_nat f) as n; intros n; clear dependent f.
     apply lookup_total_to_vals_aux.
+  Qed.
+
+  Definition valid_field f τ := 0 ≤ f < length τ.
+
+  Fixpoint tau_insert_go (τ : types) (i : nat) : types_go i τ → τ → τ :=
+    match τ, i return types_go i τ → τ → τ with
+    | Tbase X, 0%nat        => fun x _ => x
+    | Tbase _, _            => fun _ xs => xs
+    | type_nel.Tcons X _, 0%nat => fun x xs => (x, snd xs)
+    | type_nel.Tcons _ τ', S i0 => fun x xs => (fst xs, tau_insert_go τ' i0 x (snd xs))
+    end.
+
+  Definition τ_insert {τ : types} (f : Z) (x : τ !!! f) (xs : τ) : τ.
+  Proof.
+    unfold lookup_total, types_lookup_total in x.
+    revert x. case_decide.
+    - intros _. exact xs.
+    - intro x. exact (tau_insert_go τ (Z.to_nat f) x xs).
+  Defined.
+
+  Local Lemma insert_to_vals_aux {τ : types} (xs : τ) n (x : types_go n τ) :
+    to_vals (tau_insert_go τ n x xs) = <[n := #x]> (to_vals xs).
+  Proof.
+    revert xs n x.
+    induction τ as [X H | X H b IH]; intros xs n x.
+    - rewrite tapp_bind.
+      destruct n as [|n']; first reflexivity.
+      simpl. update. reflexivity.
+    - pose proof (Tcons_inv b xs) as [y [xs' ->]].
+      simpl; rewrite tapp_bind.
+      destruct n as [|n']; simpl; rewrite tapp_bind.
+      + reflexivity.
+      + rewrite IH. reflexivity.
+  Qed.
+
+  Lemma insert_to_vals {τ : types} (xs : τ) (f : Z) (x : τ !!! f) :
+    to_vals (τ_insert f x xs) = <[ f := #x ]> (to_vals xs).
+  Proof.
+    revert x.
+    unfold τ_insert, encode_types_lookup, lookup_total, types_lookup_total, insert, listz_insert.
+    case_decide as Hlt. { auto. }
+    generalize (Z.to_nat f) as n; intros n; clear dependent f.
+    intros x.
+    apply insert_to_vals_aux.
+  Qed.
+
+End types_helpers.
+
+Notation "xs !!τ f" := (τ_lookup_total f xs) (at level 20).
+Notation "<[ f τ= x ]> xs" := (τ_insert f x xs)
+  (at level 5, right associativity, format "<[  f  τ=  x  ]>  xs").
+
+Section record_resources.
+
+  Context `{!osirisGS Σ}.
+
+  Definition ownRecord {τ : types} (r : record) dq (t : mut_tag) (xs : τ) : iProp Σ :=
+    ∃ ls, isBlockLocs r ls ∗ r ⤇{dq} t ∗
+      [∗ listZ] l;v ∈ ls; (to_vals xs), l ↦{dq} v.
+
+End record_resources.
+
+Section records_reasoning.
+
+  Context `{!osirisGS Σ}.
+
+  Context {η : env} {E : coPset} {Ψ : iEff Σ}.
+
+  Lemma imp_as_record {ζ} {Φ : record → iProp Σ} (m : microvx) :
+    imp m @ E <|Ψ|> ⟨⟨ ζ ⟩⟩ {{ Φ }} -∗
+    impure E (as_record m) Ψ ζ Φ.
+  Proof.
+    iIntros "Hm".
+    iApply (imp_bind with "Hm").
+    iIntros (r) "HΦ".
+    iApply (imp_ret with "HΦ"). encode.
+  Qed.
+
+  Global Instance notval_listloc : NotVal (list loc) := {}.
+  Local Instance notval_listval : NotVal (list val) := {}.
+
+  Lemma imp_ERecord {τ : types} {ζ} (Φs : τ -#> iProp Σ) t es :
+    ⌜length τ ≤ max_array_length⌝ -∗
+    impure E (evals η es) Ψ ζ Φs -∗
+    impure E (eval η (ERecord t es)) Ψ ζ
+      (λ r, ∃ (xs : τ), ownRecord r (DfracOwn 1) t xs ∗ Φs xs).
+  Proof.
+    iIntros "%Hlength Hes". simpl_eval.
+    iApply (imp_bind with "Hes").
+    iIntros (xs) "HΦs".
+    iApply imp_bind.
+    { simpl.
+      replace (to_vals xs) with
+      (@observe (list val) (list val) (@observe_list val Encode_val) (to_vals xs)).
+      iApply (@imp_allocn _ _ _ _ _ val Encode_val (λ ls, [∗ listZ] l;v ∈ ls; (to_vals xs), l ↦ v)%I (to_vals xs)).
+      iIntros "!>" (ls) "$".
+      simpl. rewrite map_id. reflexivity. }
+    iIntros (ls) "Hls".
+    iPoseProof (big_sepLZ2_length with "Hls") as "%Hlength_ls".
+    iApply imp_bind.
+    { iApply imp_alloc_block.
+      iPureIntro. simpl.
+      rewrite Hlength_ls. rewrite to_vals_length. assumption. }
+    iIntros (r) "(Hmut & Hblocks)".
+    iApply imp_ret. encode.
+    iFrame.
   Qed.
 
   Global Instance notval_block : NotVal (mut_tag * list loc) := {}.
@@ -195,34 +245,35 @@ Section records_reasoning.
     do 2 constructor. apply Z.inhabited.(inhabitant).
   Qed.
 
-  Lemma imp_ERecordAccess {τ : types} {ζ} f {Φ : (τ !!! f) → iProp Σ} r ls e :
-    ⌜valid f ls⌝ -∗
+  Lemma imp_ERecordAccess2 {τ : types} {ζ} f {Φ : (τ !!! f) → iProp Σ} r ls e :
     ▷ isBlockLocs r ls -∗
     impure E (eval η e) Ψ ζ (λ (r' : record), ⌜r' = r⌝) -∗
     (∃ dq t (xs : τ),
-      ▷ ownRecord r dq t xs ∗
+      ▷ (⌜valid_field f τ⌝ ∗ ownRecord r dq t xs) ∗
       ▷ (ownRecord r dq t xs -∗ Φ (xs !!τ f))) -∗
     impure E (eval η (ERecordAccess e f)) Ψ ζ Φ.
   Proof.
-    iIntros "%Hvalid #Hblock He P". simpl_eval.
+    iIntros "#Hblock He P". simpl_eval.
     iApply (imp_bind with "[He]").
     { iApply (imp_as_record with "He"). }
     iIntros (?) "->".
     iDestruct "P" as
-        "(%dq & %t & %xs & P)".
-    rewrite <- (bi.later_sep (ownRecord _ _ _ _)).
-    iCombine "Hblock P" as "P".
-
+        "(%dq & %t & %xs & P1 & P2)".
+    iCombine "Hblock P1 P2" as "P".
 
     iApply (imp_bind (A1:=(mut_tag * list loc)) with "[P]").
     { iApply (imp_load_block_ghost' with "Hblock P"). }
-    iIntros ((? & ?)) "(-> & #Hblock' & Hown & HΦ) /=".
+    iIntros ((? & ?)) "(-> & #Hblock' & (%Hvalid_field & Hown) & HΦ) /=".
     iClear "Hblock".
 
     iDestruct "Hown" as "(%ls' & #Hblock & Htag & Hxs)".
     iPoseProof (isBlockLocs_valid with "Hblock' Hblock") as "->".
     iPoseProof (isBlockLocs_length with "Hblock") as "%Hlen".
     iPoseProof (big_sepLZ2_length with "Hxs") as "%Hlen_xs".
+    assert (valid f ls) as Hvalid.
+    { destruct Hvalid_field. split; first lia.
+      rewrite Hlen_xs to_vals_length. assumption. }
+
     rewrite (list_lookup_lookup_total_valid ls f Hvalid).
 
     iPoseProof (big_sepLZ2_lookup_acc _ ls (to_vals xs) f with "Hxs") as "(Hx & Hxs)".
@@ -238,6 +289,52 @@ Section records_reasoning.
     iApply "HΦ".
     iExists ls. iFrame "∗#".
     iApply ("Hxs" with "Hx").
+  Qed.
+
+  Lemma imp_ERecordSet2 {τ : types} {ζ} f {Φ : unit → iProp Σ} (Φ1 : record → iProp Σ) (Φ2 : τ !!! f → iProp Σ) e1 e2 :
+    impure E (eval η e1) Ψ ζ Φ1 -∗
+    impure E (eval η e2) Ψ ζ Φ2 -∗
+    (∀ r a, Φ1 r -∗ Φ2 a -∗
+            ∃ t (xs : τ),
+              ▷ (⌜valid_field f τ⌝ ∗ ownRecord r (DfracOwn 1) t xs) ∗
+              ▷ (ownRecord r (DfracOwn 1) t <[f τ= a]> xs -∗ Φ ())) -∗
+    impure E (eval η (ERecordSet e1 f e2)) Ψ ζ Φ.
+  Proof.
+    iIntros "He1 He2 P". simpl_eval.
+    iApply (imp_bind_par with "[He1] He2").
+    { iApply (imp_as_record with "He1"). }
+    iIntros (r a) "HΦ1 HΦ2".
+    iDestruct ("P" with "HΦ1 HΦ2") as
+        "(%j & %xs & Hown & HΦ)". iNext.
+    iDestruct "Hown" as "(%Hvalid_field & Hown)".
+    iDestruct "Hown" as "(%ls & #Hblock & Htag & Hxs)".
+    iPoseProof (isBlockLocs_length with "Hblock") as "%Hlen_ls".
+    iPoseProof (big_sepLZ2_length with "Hxs") as "%Hlen_xs".
+
+    iApply imp_bind. { iApply (imp_load_block_ghost with "Hblock"). }
+    iIntros ((t & ls')) "-> /=".
+
+    assert (valid f ls) as Hvalid.
+    { destruct Hvalid_field. split; first lia.
+      rewrite Hlen_xs to_vals_length. assumption. }
+
+    rewrite (list_lookup_lookup_total_valid ls f Hvalid).
+
+    iPoseProof (big_sepLZ2_insert_acc _ ls (to_vals xs) f with "Hxs") as "(Hx & Hxs)".
+    { apply list_lookup_lookup_total_valid. assumption. }
+    { instantiate (1:= #(xs !!τ f)).
+      transitivity (@Some val ((to_vals xs) !!! f)).
+      - apply list_lookup_lookup_total_valid.
+        rewrite <- Hlen_xs. assumption.
+      - f_equal.
+        apply lookup_total_to_vals. }
+    iApply (imp_store' with "Hx").
+    iIntros "!> Hx".
+    iApply "HΦ".
+    iExists ls. iFrame "∗#".
+    iSpecialize ("Hxs" with "Hx").
+    update. rewrite insert_to_vals.
+    iApply "Hxs".
   Qed.
 
 End records_reasoning.
